From the given information,
	\begin{align}
	\pr{E} &= \frac{3}{6} = \frac{1}{2} \\
	\pr{F} &= \frac{2}{6} = \frac{1}{3} \\	
	\pr{G} &= \frac{4}{6} = \frac{2}{3} \\	
	\pr{E F} &= \frac{1}{6}\\
	\pr{E G} &= \frac{2}{6}= \frac{1}{3}\\
	\pr{F G} &= \frac{2}{6}= \frac{1}{3}\\
	\pr{E F G} &= \frac{1}{6}
\end{align}
\begin{enumerate}
\item	
\begin{align}
	\pr{E|F} &= \frac{\pr{E F}}{\pr{F}}\\
	\pr{E|F} &= \frac{\frac{1}{6}}{\frac{1}{3}} = \frac{1}{2}\\
	\pr{F|E} &= \frac{\pr{F E}}{\pr{E}}\\
	\pr{F|E} &= \frac{\frac{1}{6}}{\frac{1}{2}} = \frac{1}{3}
	\end{align}

\item 	\begin{align}
	\pr{E|G} &= \frac{\pr{E G}}{\pr{G}}\\
	\pr{E|G} &= \frac{\frac{1}{3}}{\frac{2}{3}} = \frac{1}{2}\\
	\pr{G|E} &= \frac{\pr{G E}}{\pr{G}}\\
	\pr{G|E} &= \frac{\frac{1}{3}}{\frac{1}{2}} = \frac{2}{3}\\
	\end{align}
	
\item	%$\pr{\frac{E\cup F}{G}}$
\begin{multline}
\pr{E+F|G} = \frac{\pr{\cbrak{E+F}G}}{\pr{G}}
\\
 = \frac{\pr{EG + FG}}{\pr{G}}
\\
=\frac{\pr{EG} +\pr{ FG}- \pr{EFG}}{\pr{G}}
\\
 = \frac{3}{4}
\end{multline}
and 
\begin{align}
\pr{EF|G} = 
\frac{ \pr{EFG}}{\pr{G}}
 = \frac{1}{4}
\end{align}

\end{enumerate}
