Given,
\begin{align*}
\pr{\text {A fails}}&=\pr{A}&=0.2\\
\pr{\text{B fails alone}}&=\pr{B-A}&=0.15\\
\pr{\text{A and B fails}}&=\pr{AB}&=0.15\\
\end{align*}
 Now,we need to find \pr{\text{A fails alone}}=\pr{A-B}
\begin{enumerate}
\item
\begin{align}
    \tag{6.7.1}
    \pr{A}&=\pr{A-B}+\pr{AB}\\
    \tag{6.7.2}
    \implies \pr{A-B}&=\pr{A}-\pr{AB}\\
    \tag{6.7.3}
    \implies \pr{A-B}&=0.20-0.15\\
    \tag{6.7.4}
    \implies \pr{A-B}&=0.05
\end{align}
Therefore, \pr{\text{A fails alone}}=\pr{A-B}=0.05
\item
Now,finding the probability of B
\begin{align}
    \tag{6.7.5}
    \pr{B-A}&=\pr{B}-\pr{AB}\\
    \tag{6.7.6}
    \implies \pr{B}&=\pr{B-A}+\pr{AB}\\
    \tag{6.7.7}
    \implies \pr{B}&=0.15+0.15\\
    \tag{6.7.8}
    \implies \pr{B}&=0.30
\end{align}
Now, we need to find \pr{\text{A fails$|$B has failed}}=\pr{A|B}
\begin{align}
    \tag{6.7.9}
    \pr{A|B}&=\frac{\pr{AB}}{\pr{B}}\\
    \tag{6.7.10}
    \implies \pr{A|B}&=\frac{0.15}{0.30}\\
    \tag{6.7.11}
    \implies \pr{A|B}&=0.5
\end{align}
Therefore, \pr{\text{A fails$|$ B has failed}}=\pr{A|B}=0.5
\end{enumerate}