\begin{enumerate}[label={\roman*)}]
    \item Since the events are mutually exclusive, by definition
\begin{align}
    \pr{AB} = 0\\
    \implies \pr{A + B} = \pr{A} + \pr{B}\label{Zehahahaha}
\end{align}
On substituting the values of $\pr{A}$, $\pr{B}$ and $\pr{A+B}$ in \eqref{Zehahahaha}, we get
\begin{align}
    \cfrac{3}{5} = \cfrac{1}{2} + p\\
    \implies p = \cfrac{1}{10}
\end{align}
    \item Since the events are independent
\begin{align}
    \pr{AB} = \pr{A}\pr{B}
\end{align}
We know
\begin{align}
    \pr{A+B} = \pr{A} + \pr{B} - \pr{AB}\\
    \implies \pr{A+B} = \pr{A} + \pr{B} - \pr{A}\pr{B}\label{Gababababa}
\end{align}
On substituting the values of $\pr{A}$, $\pr{B}$ and $\pr{A+B}$ in \eqref{Gababababa}, we get
\begin{align}
    \cfrac{3}{5} = \cfrac{1}{2} + p - \cfrac{1}{2} p\\
    \implies p = \cfrac{1}{5}
\end{align}
\end{enumerate}