\begin{enumerate}[label={\roman*)}]
\item
Since the events A and B are independent events, by definition
\begin{align}
    \pr{A\, and\, B} = \pr{AB}= \pr{A}\pr{B}\label{6.15:a}
\end{align}
On substituting the values of \pr{A},\pr{B} in \eqref{6.15:a}, we get
\begin{align}
    \pr{A\, and\, B} &= \pr{A}\pr{B}\\
    &= (0.3)(0.6)\\
    \implies \pr{A\, and\, B}&=0.18
\end{align}
\item
As the events A and B are independent, then A and B' are also independent.
\begin{align}   
    \implies \pr{A\,and\,not\,B} &=\pr{AB'}\\
&= \pr{A}\pr{B'}\\
\therefore \pr{A\,and\,not\,B} &= \pr{A}\pr{B'}\label{6.15:b}
\end{align}
And we know that,
\begin{align}
    \pr{B'}=1-\pr{B}\label{6.15:c}
\end{align}
Using \eqref{6.15:c} in \eqref{6.15:b} we will get,
\begin{align}
   \pr{A\,and\,not\,B} &=\pr{AB'}\\
&= \pr{A}\pr{B'}\\
    \pr{A\,and\,not\,B} &= \pr{A}(1-\pr{B})\label{6.15:d}
\end{align}
On substituting the values of \pr{A},\pr{B} in \eqref{6.15:d}, we get
\begin{align}
    \pr{A\,and\,not\,B} &= 0.3(1-0.6)\\
    &= (0.3)(0.4)\\
    \implies \pr{A\,and\,not\,B}&= 0.12
\end{align}
\item
\begin{align}
    \pr{A\,or\,B} =\pr{A\,+\,B}\label{6.15:e}
\end{align}
We know that,
\begin{align}
    \pr{A\,+\,B} = \pr{A} + \pr{B} -\pr{AB}\label{6.15:f}
\end{align}
As events A and B are independent events,
\begin{align}
    \pr{AB}=\pr{A}\pr{B}\label{6.15:g}
\end{align}
Using \eqref{6.15:g} and \eqref{6.15:f} in \eqref{6.15:e}, We get
\begin{align}
    \pr{A\,+\,B} = \pr{A} + \pr{B} -\pr{A}\pr{B}\label{6.15:h}
\end{align}
On substituting the values of \pr{A},\pr{B} in \eqref{6.15:h}, we get
\begin{align}
    \pr{A\,or\,B} &= 0.3 + 0.6 -(0.3)(0.6)\\
    &= 0.9-0.18\\
    \implies \pr{A\,or\,B} &= 0.72\label{6.15:i}
\end{align}
\item
\begin{align}
    \pr{neither\, A\, nor\, B} &= \pr{A'B'}\\
    &=\pr{(A\,+\,B)'}\\
    \pr{neither\, A\, nor\, B}&=1-\pr{A\,+\,B}\label{6.15:j}
\end{align}
From \eqref{6.15:i},
\begin{align}
    \pr{A\,or\,B} =\pr{A\,+\,B}=0.72\label{6.15:k}
\end{align}
Using \eqref{6.15:k} in \eqref{6.15:j}, We get
\begin{align}
    \pr{neither\, A\, nor\, B}&=1-0.72\\
   \implies \pr{neither\, A\, nor\, B}&=0.28
\end{align}
\end{enumerate}