%
\begin{align}
    E(X) &= \frac{1}{\sqrt{2\pi}} \int_{-\infty}^{\infty} x e^{-\frac{x^2}{2}}dx\\
    &=0 \quad \brak{ \text{ odd function}}
\end{align}
\begin{align}
    E\brak{X^2}&= \frac{1}{\sqrt{2\pi}}\int_{-\infty}^{\infty} x^2
e^ {-\frac{x^2}{2}} dx \quad \brak{even function}\\
    &= \frac{2}{\sqrt{2\pi}} \int_{0}^{\infty} x^2 e^{-\frac{x^2}{2}} dx\\
    &= \frac{2}{\sqrt{2\pi}}\int_{0}^{\infty}\sqrt{2u}e^{-u} du \quad\brak{Let \frac{x^2}{2}= u}\\
    &= \frac{2}{\sqrt{\pi}} \int_{0}^{\infty} e^{-u} u^{\frac{3}{2}-1} du\\
    &= \frac{2}{\sqrt{\pi}} \Gamma\brak{{\frac{3}{2}}}\\
    &= \frac{1}{\sqrt{\pi}}\Gamma\brak{\frac{1}{2}} \\
    &= 1
\end{align}
where we have used the fact that
\begin{align}
\quad\because \Gamma(n)= (n-1)\Gamma(n-1); \Gamma\brak{\frac{1}{2}}=\sqrt{\pi}
\end{align}
%
Thus, the  variance is
\begin{align}
    \sigma^2 =  E\brak X^2 - E^2\brak X = 1
\end{align}
